added verification for add method

rangePackBeforeCall.bpl
@@ -1,30 +1,20 @@
-//The name of this class is Link.
 type Ref;
-type FractionRangeType = [int, int, Ref] real;
-type PackedRangeType = [int, int, Ref] bool;
 
 const null : Ref;
 
 var val : [Ref]int;
 var next : [Ref]Ref;
 
-var fracRange : FractionRangeType;
-var packedRange : PackedRangeType;
+var fracRange : [int, int, Ref] real;
+var packedRange : [int, int, Ref] bool;
+var fracUniRange : [Ref] real;
+var packedUniRange : [int, int, Ref] bool;
 
 
 procedure ConstructLink(x: int, y:int, val1: int, next1: Ref, this: Ref);
 	ensures (val[this] == val1) && 
 		(next[this] == next1);
 
-// We assume that packedRange[x,y, next[this]] holds
-// because it is the invariant
-// so we do not need to add it in the requires of PackRange.
-// How do we know that this is the invariant for next[this]?
-// We do not need to have packedRange[x,y,next[this]]
-// in the requires.
-// When you unpack something, you assume that all the object propositions inside it are packed. 
-// That's why we need the ensures packedRange[] there. It is like an assume.
-// When you pack something, you need just a fraction, so you don't actually need the requires packedRange[].
 procedure PackRange(x:int, y:int, this:Ref);
 	requires (val[this] >= x);
 	requires (val[this] <= y);
@@ -45,26 +35,56 @@ procedure PackUniRange(x:int, y:int, this:Ref);
 	requires (val[this] >= x);
 	requires (val[this] <= y);
 	requires ((next[this] == null) ||
-		  (fracRange[x,y,next[this]] == 1.0) );
+		  (fracUniRange[next[this]] == 1.0) );
 
 procedure UnpackUniRange(x:int, y:int, this:Ref);
-	requires packedRange[x,y,this];
-	requires (fracRange[x,y,this] > 0.0);
+	requires packedUniRange[x,y,this];
+	requires (fracUniRange[this] > 0.0);
 	ensures  (val[this] >= x) &&
 		 (val[this] <= y) &&
 		 ((next[this] == null) ||
 		  (
-		  (fracRange[x,y,next[this]] == 1.0) )
+		  (fracUniRange[next[this]] == 1.0) )
 		 );
+
+procedure add(z:int, x:int, y:int, this: Ref)
+	modifies val, packedUniRange, fracUniRange;
+	requires x < y;
+  //Could let only packed[] to have x,y,this as parameters
+  //and frac could only have this
+	requires fracUniRange[this] == 1.0;
+  requires (forall x1:int, y1:int, x0:Ref :: packedUniRange[x1,y1,x0]);
+	ensures packedUniRange[x+z,y+z,this];
+	ensures fracUniRange[this] == 1.0;
+	ensures (forall x1:int, y1:int, x0:Ref :: packedUniRange[x1,y1,x0]);
+{
+	call UnpackUniRange(x, y, this);
+	packedUniRange[x,y,this] := false;
+ //Might need to add back the params[] idea
+ //because packedUniRange above is left unpacked for x,y
+
+	val[this] := val[this]+z;
   
-procedure addModulo11(x:int, this: Ref);
+  //This holds because this was holding before the assignment:
+  //	fracUniRange[x,y,next[this]] := 1.0;
+  fracUniRange[next[this]] := 1.0;
+  call PackUniRange(x+z, y+z, this);
+	packedUniRange[x+z,y+z,this] := true;
+	fracUniRange[next[this]] :=  1.0;
+	
+	if (next[this] != null )
+	{ 
+    		call add(z, x, y, next[this]);
+	}
+}
+  
+procedure addModulo11(x:int, this: Ref) 
 	modifies val, packedRange, fracRange;
 	requires x >= 0;
 	requires fracRange[0,10,this] > 0.0;
-  	requires (forall y:Ref :: (packedRange[0,10,y] == true));
+  requires (forall y:Ref :: (packedRange[0,10,y] == true));
 	ensures packedRange[0,10,this];
 	ensures fracRange[0,10,this] > 0.0;
-	//This says that Range is an invariant of all the objects in this method.
 	ensures (forall y:Ref :: (packedRange[0,10,y] == old(packedRange[0,10,y])) );
 	ensures (forall y:Ref :: (fracRange[0,10,y] == old(fracRange[0,10,y])) );
 {
@@ -80,51 +100,10 @@ procedure addModulo11(x:int, this: Ref);
 	
 	if (next[this] != null )
 	{ 
-    		call addModulo11(x, next[this]);
+    
+		call addModulo11(x, next[this]);
 		fracRange[0,10,next[this]] := fracRange[0,10,next[this]] * 2.0;
 		fracRange[0,10,next[this]] := fracRange[0,10,next[this]] / 2.0;
-	}
-}
-
-    void add(int z)
-    int x, int y: //SpecExpression with list of declaration
-    requires x < y && (this#1 UniRange(x,y))
-    ensures (this#1 UniRange(x+z,y+z))
-    {
-    	unpack(this#1 UniRange(x,y));
-    	this.val = this.val + z;
-    	pack(this#1 UniRange(x+z,y+z));
-    	if (this.next != null) {
-    		this.next.add(z);
-    	}
-    }
-
-procedure add(z:int, x:int, y:int, this: Ref);
-	modifies val, packedRange, fracRange;
-	requires x < y;
-	requires fracUniRange[x,y,this] > 0.0;
-  	requires (forall x0:Ref :: (packedUniRange[x,y,x0] == true));
-	ensures packedUniRange[x,y,this];
-	ensures fracUniRange[x,y,this] > 0.0;
-	//This says that Range is an invariant of all the objects in this method.
-	ensures (forall x0:Ref :: (packedUniRange[x,y,x0] == old(packedUniRange[x,y,x0])) );
-	ensures (forall x0:Ref :: (fracUniRange[x,y,x0] == old(fracUniRange[x,y,x0])) );
-{
-	call UnpackUniRange(x, y, this);
-	packedUniRange[x,y,this] := false;
-	fracUniRange[x,y,next[this]] := fracRange[x,y,next[this]] * 2.0;
-
-	val[this] := modulo((val[this]+x),11);
-  
-  	call PackUniRange(0, 10, this);
-	packedRange[0,10,this] := true;
-	fracRange[0,10,next[this]] := fracRange[0,10,next[this]] / 2.0;
-	
-	if (next[this] != null )
-	{ 
-    		call add(z, x, y, next[this]);
-		fracUniRange[0,10,next[this]] := fracUniRange[0,10,next[this]] * 2.0;
-		fracUniRange[0,10,next[this]] := fracUniRange[0,10,next[this]] / 2.0;
 	}
 }
 
@@ -142,13 +121,11 @@ axiom (forall x:int, y:int :: {modulo(x,y)}
 
 procedure main()
 	modifies val, packedRange, fracRange;
-   	requires (forall y:Ref :: (packedRange[0,10,y] == true));
+   requires (forall y:Ref :: (packedRange[0,10,y] == true));
 {
 	var l1 : Ref;
 	var l2 : Ref;
 	var l3 : Ref;
-	//Need to state that l1 satisfies the Range predicate.
-	//TODO need to add fraction manipulation
 	call ConstructLink(0, 10, 3, null, l1);
 	packedRange[0,10,l1] := true;
 	fracRange[0,10,l1] := 1.0;
@@ -165,6 +142,7 @@ procedure main()
 
 	call addModulo11(20, l3); 
 }
+
 
 
 
